it passes!

tttree.dfy
@@ -1,9 +1,17 @@
+type Key = int
+
+predicate method key_lt(a: Key, b: Key)
+	ensures key_lt(a, b) ==> a != b;
+{
+	a < b
+}
+
 datatype Node<Value> =
-	Leaf(key: int, value: Value) |
-	TwoNode(left: Node, pivot: int,
+	Leaf(key: Key, value: Value) |
+	TwoNode(left: Node, pivot: Key,
 	        right: Node) |
-	ThreeNode(left: Node, pivota: int,
-	          middle: Node, pivotb: int,
+	ThreeNode(left: Node, pivota: Key,
+	          middle: Node, pivotb: Key,
 						right: Node)
 
 function merge_maps<U,T>(mapa: map<U,T>, mapb: map<U,T>) : map<U,T>
@@ -18,8 +26,18 @@ function merge_maps<U,T>(mapa: map<U,T>, mapb: map<U,T>) : map<U,T>
 	map x : U | (x in mapa.Keys + mapb.Keys) :: if x in mapa then mapa[x] else mapb[x]
 }
 
+function SubtreeAllKeys(tree: Node) : set<Key>
+{
+	match tree {
+		case Leaf(key, value) => {key}
+		case TwoNode(left, pivot, right) => SubtreeAllKeys(left) + {pivot} + SubtreeAllKeys(right)
+		case ThreeNode(left, pivota, middle, pivotb, right) =>
+			SubtreeAllKeys(left) + {pivota} + SubtreeAllKeys(middle) + {pivotb} + SubtreeAllKeys(right)
+	}
+}
+
 function SubtreeContents<Value>(tree: Node<Value>) : map<int, Value>
-	ensures SubtreeContents(tree).Keys != {};
+	ensures SubtreeContents(tree).Keys <= SubtreeAllKeys(tree);
 {
 	if tree.Leaf? then
 		var r := map[tree.key := tree.value];
@@ -34,33 +52,31 @@ function SubtreeContents<Value>(tree: Node<Value>) : map<int, Value>
 }
 
 predicate ContentsAreLessThan(tree: Node, pivot: int) {
-	forall lv :: lv in SubtreeContents(tree).Keys ==> lv < pivot
+	forall lv :: lv in SubtreeAllKeys(tree) ==> key_lt(lv, pivot)
 }
 
 predicate ContentsAreGreaterEqualThan(pivot: int, tree: Node) {
-	forall lv :: lv in SubtreeContents(tree).Keys ==> lv >= pivot
+	forall lv :: lv in SubtreeAllKeys(tree) ==> !key_lt(lv, pivot)
 }
 
 predicate OrderedTree(tree: Node) {
-    if tree.Leaf?
-			then SubtreeContents(tree).Keys != {}
-		else if tree.TwoNode?
-      then
-			ContentsAreLessThan(tree.left, tree.pivot) &&
-			ContentsAreGreaterEqualThan(tree.pivot, tree.right) &&
-			SubtreeContents(tree).Keys != {} &&
-			OrderedTree(tree.left) &&
-			OrderedTree(tree.right)
-		else
-			tree.pivota < tree.pivotb &&
-			ContentsAreLessThan(tree.left, tree.pivota) &&
-			ContentsAreGreaterEqualThan(tree.pivota, tree.middle) &&
-			ContentsAreLessThan(tree.middle, tree.pivotb) &&
-			ContentsAreGreaterEqualThan(tree.pivotb, tree.right) &&
-			SubtreeContents(tree).Keys != {} &&
-			OrderedTree(tree.left) &&
-			OrderedTree(tree.middle) &&
-			OrderedTree(tree.right)
+  if tree.Leaf?
+		then true
+	else if tree.TwoNode?
+    then
+		ContentsAreLessThan(tree.left, tree.pivot) &&
+		ContentsAreGreaterEqualThan(tree.pivot, tree.right) &&
+		OrderedTree(tree.left) &&
+		OrderedTree(tree.right)
+	else
+		key_lt(tree.pivota, tree.pivotb) &&
+		ContentsAreLessThan(tree.left, tree.pivota) &&
+		ContentsAreGreaterEqualThan(tree.pivota, tree.middle) &&
+		ContentsAreLessThan(tree.middle, tree.pivotb) &&
+		ContentsAreGreaterEqualThan(tree.pivotb, tree.right) &&
+		OrderedTree(tree.left) &&
+		OrderedTree(tree.middle) &&
+		OrderedTree(tree.right)
 }
 
 function min(a: int, b: int) : int
@@ -127,9 +143,37 @@ function Height(tree: Node) : int
 	minHeight(tree)
 }
 
+function method mkTwoNode(t1: Node, pivot: Key, t2: Node) : Node
+	requires TTSubtree(t1);
+	requires TTSubtree(t2);
+	requires Height(t1) == Height(t2);
+	requires ContentsAreLessThan(t1, pivot);
+	requires ContentsAreGreaterEqualThan(pivot, t2);
+	ensures TTSubtree(mkTwoNode(t1, pivot, t2));
+	ensures Height(mkTwoNode(t1, pivot, t2)) == Height(t1) + 1;
+{
+	TwoNode(t1, pivot, t2)
+}
+
+function method mkThreeNode(t1: Node, pivota: Key, t2: Node, pivotb: Key, t3: Node) : Node
+	requires TTSubtree(t1);
+	requires TTSubtree(t2);
+	requires TTSubtree(t3);
+	requires Height(t1) == Height(t2) == Height(t3);
+	requires key_lt(pivota, pivotb);
+	requires ContentsAreLessThan(t1, pivota);
+	requires ContentsAreGreaterEqualThan(pivota, t2);
+	requires ContentsAreLessThan(t2, pivotb);
+	requires ContentsAreGreaterEqualThan(pivotb, t3);
+	ensures TTSubtree(mkThreeNode(t1, pivota, t2, pivotb, t3));
+	ensures Height(mkThreeNode(t1, pivota, t2, pivotb, t3)) == Height(t1) + 1;
+{
+	ThreeNode(t1, pivota, t2, pivotb, t3)
+}
+
 datatype QueryResult<Value> = KeyDoesNotExist | ValueForKey(value: Value)
 
-function method QuerySubtree<Value>(tree: Node<Value>, key: int) : QueryResult<Value>
+function method QuerySubtree<Value>(tree: Node<Value>, key: Key) : QueryResult<Value>
     requires OrderedTree(tree);
     ensures QuerySubtree(tree, key) == KeyDoesNotExist <==>
 			(key !in SubtreeContents(tree));
@@ -140,105 +184,109 @@ function method QuerySubtree<Value>(tree: Node<Value>, key: int) : QueryResult<V
 		ValueForKey(tree.value)
 	else if tree.Leaf? && tree.key != key then
 		KeyDoesNotExist
-	else if tree.TwoNode? && key < tree.pivot then
+	else if tree.TwoNode? && key_lt(key, tree.pivot) then
 		QuerySubtree(tree.left, key)
-	else if tree.TwoNode? && key >= tree.pivot then
+	else if tree.TwoNode? && !key_lt(key, tree.pivot) then
 		QuerySubtree(tree.right, key)
-	else if tree.ThreeNode? && key < tree.pivota then
+	else if tree.ThreeNode? && key_lt(key, tree.pivota) then
 		QuerySubtree(tree.left, key)
-	else if tree.ThreeNode? && key < tree.pivotb then
+	else if tree.ThreeNode? && key_lt(key, tree.pivotb) then
 		QuerySubtree(tree.middle, key)
 	else
 		QuerySubtree(tree.right, key)
 }
 
-// function minElementOfSubtree(tree: Node) : int
-// 	requires(OrderedTree(tree));
-// 	ensures(forall x :: x in SubtreeContents(tree) ==> x >= minElementOfSubtree(tree));
-// {
-// 	if tree.Leaf? then tree.key
-// 	else minElementOfSubtree(tree.left)
-// }
+// // function minElementOfSubtree(tree: Node) : int
+// // 	requires(OrderedTree(tree));
+// // 	ensures(forall x :: x in SubtreeContents(tree) ==> x >= minElementOfSubtree(tree));
+// // {
+// // 	if tree.Leaf? then tree.key
+// // 	else minElementOfSubtree(tree.left)
+// // }
 
-// function maxElementOfSubtree(tree: Node) : int
-// 	requires(OrderedTree(tree));
-// 	ensures(forall x :: x in SubtreeContents(tree) ==> x <= maxElementOfSubtree(tree));
-// {
-// 	if tree.Leaf? then tree.key
-// 	else maxElementOfSubtree(tree.right)
-// }
+// // function maxElementOfSubtree(tree: Node) : int
+// // 	requires(OrderedTree(tree));
+// // 	ensures(forall x :: x in SubtreeContents(tree) ==> x <= maxElementOfSubtree(tree));
+// // {
+// // 	if tree.Leaf? then tree.key
+// // 	else maxElementOfSubtree(tree.right)
+// // }
 
 datatype InsertionResult<Value> = InsertionResult(tree: Node<Value>, split: bool)
 	
-method InsertIntoSubtree<Value>(tree: Node<Value>, key: int, value: Value)
+method InsertIntoSubtree<Value>(tree: Node<Value>, key: Key, value: Value)
 	returns (result: InsertionResult<Value>)
 	requires TTSubtree(tree);
 	ensures TTSubtree(result.tree);
+	ensures SubtreeAllKeys(result.tree) == SubtreeAllKeys(tree) + {key};
 	ensures SubtreeContents(result.tree) == SubtreeContents(tree)[key := value];
-	ensures result.split ==> Height(result.tree) == Height(tree) + 1;
 	ensures result.split ==> result.tree.TwoNode?;
+	ensures result.split ==> result.tree.pivot in SubtreeAllKeys(tree) + {key};
+	ensures result.split ==> Height(result.tree) == Height(tree) + 1;
 	ensures !result.split ==> Height(result.tree) == Height(tree);
 {
 	if tree.Leaf? {
 		if tree.key == key {
 			result := InsertionResult(Leaf(key, value), false);
-		} else if tree.key < key {
+		} else if key_lt(tree.key, key) {
 			var newright := Leaf(key, value);
-			var newtree := TwoNode(tree, key, newright);
+			var newtree := mkTwoNode(tree, key, newright);
 			assert(Height(newright) == Height(tree));
 			assert(Height(newtree) == Height(tree) + 1);
 			result := InsertionResult(newtree, true);
 		} else {
 			var newleft := Leaf(key, value);
-			var newtree := TwoNode(newleft, tree.key, tree);
+			var newtree := mkTwoNode(newleft, tree.key, tree);
 			assert(Height(newleft) == Height(tree));
 			assert(Height(newtree) == Height(tree) + 1);
 			result := InsertionResult(newtree, true);
 		}
 	} else if tree.TwoNode? {
-		if key < tree.pivot {
+		if key_lt(key, tree.pivot) {
 			var subresult := InsertIntoSubtree(tree.left, key, value);
 			if !subresult.split {
-				result := InsertionResult(TwoNode(subresult.tree, tree.pivot, tree.right), false);
+				result := InsertionResult(mkTwoNode(subresult.tree, tree.pivot, tree.right), false);
 			} else {
-				result := InsertionResult(ThreeNode(subresult.tree.left, subresult.tree.pivot,
-					                                 subresult.tree.right, tree.pivot,
-																					 tree.right), false);
+				assert SubtreeAllKeys(subresult.tree.right) != {};
+				assert key_lt(subresult.tree.pivot, tree.pivot);
+				result := InsertionResult(mkThreeNode(subresult.tree.left, subresult.tree.pivot,
+					                                   subresult.tree.right, tree.pivot,
+																					   tree.right), false);
 			}
 		} else {
 			var subresult := InsertIntoSubtree(tree.right, key, value);
 			if !subresult.split {
-				result := InsertionResult(TwoNode(tree.left, tree.pivot, subresult.tree), false);
+				result := InsertionResult(mkTwoNode(tree.left, tree.pivot, subresult.tree), false);
 			} else {
-				result := InsertionResult(ThreeNode(tree.left, tree.pivot,
-			                		                  subresult.tree.left, subresult.tree.pivot,
-																						subresult.tree.right), false);
+				result := InsertionResult(mkThreeNode(tree.left, tree.pivot,
+			                		                   subresult.tree.left, subresult.tree.pivot,
+																						 subresult.tree.right), false);
 			}
 		}
 	} else if tree.ThreeNode? {
-		if key < tree.pivota {
+		if key_lt(key, tree.pivota) {
 			var subresult := InsertIntoSubtree(tree.left, key, value);
 			if !subresult.split {
-				result := InsertionResult(ThreeNode(subresult.tree, tree.pivota,
-					                                  tree.middle, tree.pivotb,
-																						tree.right), false);
+				result := InsertionResult(mkThreeNode(subresult.tree, tree.pivota,
+					                                   tree.middle, tree.pivotb,
+																						 tree.right), false);
 			} else {
-				var newright := TwoNode(tree.middle, tree.pivotb, tree.right);
+				var newright := mkTwoNode(tree.middle, tree.pivotb, tree.right);
 				assert(Height(newright) == Height(tree));
-				var newtree := TwoNode(subresult.tree, tree.pivota, newright);
+				var newtree := mkTwoNode(subresult.tree, tree.pivota, newright);
 				assert(Height(newtree) == Height(tree) + 1);
 				result := InsertionResult(newtree, true);
 			}
-		} else if key < tree.pivotb {
+		} else if key_lt(key, tree.pivotb) {
 			var subresult := InsertIntoSubtree(tree.middle, key, value);
 			if !subresult.split {
-				result := InsertionResult(ThreeNode(tree.left, tree.pivota,
-					                                  subresult.tree, tree.pivotb,
-																						tree.right), false);
+				result := InsertionResult(mkThreeNode(tree.left, tree.pivota,
+					                                   subresult.tree, tree.pivotb,
+																						 tree.right), false);
 			} else {
-				var newleft := TwoNode(tree.left, tree.pivota, subresult.tree.left);
-				var newright := TwoNode(subresult.tree.right, tree.pivotb, tree.right);
-				var newtree := TwoNode(newleft, subresult.tree.pivot, newright);
+				var newleft := mkTwoNode(tree.left, tree.pivota, subresult.tree.left);
+				var newright := mkTwoNode(subresult.tree.right, tree.pivotb, tree.right);
+				var newtree := mkTwoNode(newleft, subresult.tree.pivot, newright);
 				assert(Height(newleft) == Height(tree));
 				assert(Height(newright) == Height(tree));
 				assert(Height(newtree) == Height(tree) + 1);
@@ -247,9 +295,9 @@ method InsertIntoSubtree<Value>(tree: Node<Value>, key: int, value: Value)
 		} else {
 			var subresult := InsertIntoSubtree(tree.right, key, value);
 			if !subresult.split {
-				result := InsertionResult(ThreeNode(tree.left, tree.pivota,
-					                                  tree.middle, tree.pivotb,
-																						subresult.tree), false);
+				result := InsertionResult(mkThreeNode(tree.left, tree.pivota,
+					                                   tree.middle, tree.pivotb,
+																						 subresult.tree), false);
 			} else {
 				var newleft := TwoNode(tree.left, tree.pivota, tree.middle);
 				var newtree := TwoNode(newleft, tree.pivotb, subresult.tree);
@@ -261,70 +309,70 @@ method InsertIntoSubtree<Value>(tree: Node<Value>, key: int, value: Value)
 	} 
 }
 
-datatype Tree<Value> = EmptyTree | NonEmptyTree(root: Node<Value>)
+// // datatype Tree<Value> = EmptyTree | NonEmptyTree(root: Node<Value>)
 		
-predicate TTTree<Value>(tree: Tree<Value>) {
-	tree.EmptyTree? || TTSubtree(tree.root)
-}
+// // predicate TTTree<Value>(tree: Tree<Value>) {
+// // 	tree.EmptyTree? || TTSubtree(tree.root)
+// // }
 
-function Contents<Value>(tree: Tree<Value>) : map<int, Value>
-{
-	if tree.EmptyTree?
-		then map[]
-	else
-		SubtreeContents(tree.root)
-}
+// // function Contents<Value>(tree: Tree<Value>) : map<int, Value>
+// // {
+// // 	if tree.EmptyTree?
+// // 		then map[]
+// // 	else
+// // 		SubtreeContents(tree.root)
+// // }
 
-function method Query<Value>(tree: Tree<Value>, key: int) : QueryResult<Value>
-	requires(TTTree(tree));
-  ensures Query(tree, key) == KeyDoesNotExist <==>
-		(key !in Contents(tree));
-  ensures Query(tree, key).ValueForKey? <==>
-		(key in Contents(tree) && Contents(tree)[key] == Query(tree, key).value);
-{
-	if tree.EmptyTree? then
-		KeyDoesNotExist
-	else
-		QuerySubtree(tree.root, key)
-}
-
-method Insert<Value>(tree: Tree<Value>, key: int, value: Value) returns (newtree: Tree<Value>)
-	requires TTTree(tree);
-	ensures TTTree(newtree);
-	ensures Contents(newtree) == Contents(tree)[key := value];
-	ensures newtree.NonEmptyTree?;
-{
-	if tree.EmptyTree? {
-		newtree := NonEmptyTree(Leaf(key, value));
-	} else {
-		var result := InsertIntoSubtree(tree.root, key, value);
-		newtree := NonEmptyTree(result.tree);
-	}
-}
-
-// // datatype DeletionResult = DeletionResult(tree: Tree, merged: bool)
-	
-// // function DeleteFromSubtree(tree: Tree, key: int) : DeletionResult
-// // 	requires TTTree(tree);
-// // 	ensures TTTree(result.tree);
-// // 	ensures Contents(result.tree) == Contents(tree) - {key};
+// // function method Query<Value>(tree: Tree<Value>, key: int) : QueryResult<Value>
+// // 	requires(TTTree(tree));
+// //   ensures Query(tree, key) == KeyDoesNotExist <==>
+// // 		(key !in Contents(tree));
+// //   ensures Query(tree, key).ValueForKey? <==>
+// // 		(key in Contents(tree) && Contents(tree)[key] == Query(tree, key).value);
 // // {
 // // 	if tree.EmptyTree? then
-// // 		DeletionResult(EmptyTree, false)
+// // 		KeyDoesNotExist
 // // 	else
-// // 		match tree.root {
-// // 			case Leaf(v) =>
-// // 				if v == key then DeletionResult(EmptyTree, true)
-// // 				else DeletionResult(tree, false)
-// // 			case TwoNode(left, pivot, right) =>
-// // 				if key < pivot then {
-// // 					var subresult := DeleteFromSubtree(left, key);
-// // 					if !subresult.merged then
-// // 						DeletionResult(NonEmptyTree(subresult.root, tree.root.pivot, tree.root.right))
-// // 					else
-						
-// // 				} else {
-// // 				}
-// // 		}
+// // 		QuerySubtree(tree.root, key)
 // // }
+
+// // method Insert<Value>(tree: Tree<Value>, key: int, value: Value) returns (newtree: Tree<Value>)
+// // 	requires TTTree(tree);
+// // 	ensures TTTree(newtree);
+// // 	ensures Contents(newtree) == Contents(tree)[key := value];
+// // 	ensures newtree.NonEmptyTree?;
+// // {
+// // 	if tree.EmptyTree? {
+// // 		newtree := NonEmptyTree(Leaf(key, value));
+// // 	} else {
+// // 		var result := InsertIntoSubtree(tree.root, key, value);
+// // 		newtree := NonEmptyTree(result.tree);
+// // 	}
+// // }
+
+// // // // datatype DeletionResult = DeletionResult(tree: Tree, merged: bool)
+	
+// // // // function DeleteFromSubtree(tree: Tree, key: int) : DeletionResult
+// // // // 	requires TTTree(tree);
+// // // // 	ensures TTTree(result.tree);
+// // // // 	ensures Contents(result.tree) == Contents(tree) - {key};
+// // // // {
+// // // // 	if tree.EmptyTree? then
+// // // // 		DeletionResult(EmptyTree, false)
+// // // // 	else
+// // // // 		match tree.root {
+// // // // 			case Leaf(v) =>
+// // // // 				if v == key then DeletionResult(EmptyTree, true)
+// // // // 				else DeletionResult(tree, false)
+// // // // 			case TwoNode(left, pivot, right) =>
+// // // // 				if key < pivot then {
+// // // // 					var subresult := DeleteFromSubtree(left, key);
+// // // // 					if !subresult.merged then
+// // // // 						DeletionResult(NonEmptyTree(subresult.root, tree.root.pivot, tree.root.right))
+// // // // 					else
+						
+// // // // 				} else {
+// // // // 				}
+// // // // 		}
+// // // // }
 
